src/Iris/Std/Namespaces.lean
@@ -13,11 +13,13 @@ instance : Pos.Countable Namespace := by infer_instance
 
 def nroot : Namespace := List.nil
 
+open Iris.Std.CoPset
+
 def ndot [Pos.Countable A] (N : Namespace) (x : A) : Namespace :=
   (Pos.Countable.encode x) :: N
 
 def nclose (N : Namespace) : CoPset :=
-  CoPset.suffixes ((Pos.flatten N))
+  suffixes ((Pos.flatten N))
 
 instance : CoeOut Namespace CoPset where coe := nclose
 
@@ -26,12 +28,12 @@ infix:80 ".@" => ndot
 instance ndisjoint : Iris.Std.Disjoint Namespace where
   disjoint N1 N2 := nclose N1 ## nclose N2
 
-theorem nclose_root : ↑nroot = CoPset.full := by rfl
+theorem nclose_root : ↑nroot = full := by rfl
 
 theorem nclose_subseteq [Pos.Countable A] N (x : A) : (↑N.@x : CoPset) ⊆ (↑N : CoPset) := by
   intros p
   simp [nclose, ndot]
-  rewrite [CoPset.elem_suffixes]; rewrite [CoPset.elem_suffixes]
+  rewrite [elem_suffixes]; rewrite [elem_suffixes]
   rintro ⟨ q, Heq ⟩; rewrite [Heq]
   obtain ⟨ q', Heq ⟩ :=
     (Pos.flatten_suffix N (ndot N x) (by exists [Pos.Countable.encode x]))
@@ -41,14 +43,14 @@ theorem nclose_subseteq [Pos.Countable A] N (x : A) : (↑N.@x : CoPset) ⊆ (�
 
 theorem nclose_subseteq' [Pos.Countable A] E (N : Namespace) (x : A) : (↑N : CoPset) ⊆ E -> (↑(N.@x) : CoPset) ⊆ E := by
   intro Hsubset
-  apply CoPset.subseteq_trans
+  apply subseteq_trans
   apply nclose_subseteq
   assumption
 
 theorem ndot_ne_disjoint [Pos.Countable A] (N : Namespace) (x y : A) :
   x ≠ y -> N.@x ## N.@y := by
   intros Hxy p; simp [nclose];
-  rewrite [CoPset.elem_suffixes]; rewrite [CoPset.elem_suffixes]
+  rewrite [elem_suffixes]; rewrite [elem_suffixes]
   rintro ⟨ qx, Heqx ⟩; rintro ⟨ qy, Heqy ⟩
   rewrite [Heqx] at Heqy
   have := Pos.flatten_suffix_eq qx qy (N.@x) (N.@y) (by simp [ndot]) Heqy
@@ -59,8 +61,8 @@ theorem ndot_ne_disjoint [Pos.Countable A] (N : Namespace) (x y : A) :
 theorem ndot_preserve_disjoint_l [Pos.Countable A] (N : Namespace) (E : CoPset) (x : A) :
   ↑N ## E → ↑(N.@x) ## E := by
   have := nclose_subseteq N x
-  simp [Iris.Std.disjoint]; simp [Subset] at this
-  intros Hdisj p; exact fun a_1 => Hdisj p (this p a_1)
+  intros Hdisj p
+  exact fun a_1 => Hdisj p (this p a_1)
 
 theorem ndot_preserve_disjoint_r [Pos.Countable A] (N : Namespace) (E : CoPset) (x : A) :
   E ## ↑N → E ## ↑(N.@x) := by
