src/Iris/Algebra/CoPset.lean
@@ -1,0 +1,213 @@
+import Iris.Algebra.CMRA
+import Iris.Algebra.OFE
+import Iris.Std.Positives
+import Iris.Std.CoPset
+
+open Iris
+
+open OFE CMRA UCMRA
+open Std.CoPset
+
+inductive CoPsetDisj where
+  | copset : CoPset → CoPsetDisj
+  | copset_invalid : CoPsetDisj
+
+abbrev CoPsetDisjO := LeibnizO CoPsetDisj
+
+abbrev copset : CoPset → CoPsetDisjO := fun X => .mk (.copset X)
+
+instance : OFE CoPsetDisjO := inferInstance
+
+namespace CoPset
+
+def unit : CoPsetDisjO := .mk (.copset ∅)
+
+def pcore : CoPsetDisjO → Option CoPsetDisjO := fun _ => some unit
+
+def op (x y : CoPsetDisjO) : CoPsetDisjO :=
+  match x.car, y.car with
+  | .copset x, .copset y => if (x ## y) then .mk (.copset (x ∪ y)) else .mk .copset_invalid
+  | _, _ => .mk .copset_invalid
+
+def valid (x : CoPsetDisjO) : Prop :=
+  match x.car with
+  | .copset _ => True
+  | _ => False
+
+theorem unit_valid : valid unit := by simp [unit, valid]
+
+def validN : Nat → CoPsetDisjO → Prop := fun _ x => valid x
+
+instance op_ne : OFE.NonExpansive (op x) where
+  ne n y z H := by rw [H]
+
+theorem pcore_ne : x ≡{n}≡ y → pcore x = some cx →
+    ∃ cy, pcore y = some cy ∧ cx ≡{n}≡ cy := by
+    intro H1 H2
+    exists cx
+
+theorem validN_ne : x ≡{n}≡ y → validN n x → validN n y := by
+  intro H G; rw [<-H]; assumption
+
+theorem valid_iff_validN : valid x ↔ ∀ n, validN n x := by
+  apply Iff.intro
+  · intro H n; apply H
+  · intro H; apply H 0
+
+theorem validN_succ : validN n.succ x → validN n x := by
+  intro H; apply H
+
+theorem validN_op_left : validN n (op x y) → validN n x := by
+  rcases x, y with ⟨⟨⟨x⟩ | _⟩, ⟨⟨y⟩ | _⟩⟩ <;> simp [op, validN, valid]
+
+theorem assoc : op x (op y z) ≡ op (op x y) z := by
+  rcases x, y, z with ⟨⟨⟨x⟩ | _⟩, ⟨⟨y⟩ | _⟩, ⟨⟨z⟩ | _⟩⟩ <;> simp [op]
+  if H : y ## z
+  then
+    simp [H]
+    if G : x ## y
+    then
+      simp [G]
+      if J : x ## z
+      then
+        have K1 : x ## y ∪ z := by
+          symm
+          rw [disj_union]; apply And.intro <;> (symm; assumption)
+        have K2 : x ∪ y ## z := by
+          rw [disj_union]; apply And.intro <;> assumption
+        simp [K1, K2]
+        rw [Iris.Std.Associative.assoc (R := Eq) (α := CoPset) (f := Union.union)]
+      else
+        have K1 : ¬ x ## y ∪ z := by
+          intro C
+          symm at C; rw [disj_union] at C
+          apply J; symm; exact C.right
+        have K2 : ¬ x ∪ y ## z := by
+          rw [disj_union, not_and]
+          intro C
+          exfalso; apply J C
+        simp [K1, K2]
+    else
+      simp [G]
+      intro C; symm at C; rw [disj_union] at C
+      apply (G (disj_symm _ _ C.left))
+  else
+    simp [H]
+    if G : x ## y
+    then
+      simp [G]
+      intro C; apply H
+      rw [disj_union] at C
+      apply C.right
+    else
+      simp [G]
+
+theorem comm : op x y ≡ op y x := by
+  rcases x, y with ⟨⟨⟨x⟩ | _⟩, ⟨⟨y⟩ | _⟩⟩ <;> simp [op]
+  if H : x ## y
+  then
+    have H' : y ## x := by symm; assumption
+    simp [H, H', Iris.Std.Commutative.comm (R := Eq) (α := CoPset) (f := Union.union)]
+  else simp [H]
+       intro c; apply H (disj_symm _ _ c)
+
+theorem pcore_op_left : pcore x = some cx → op cx x ≡ x := by
+  rcases x with ⟨x | _⟩ <;> rcases cx with ⟨cx | _⟩ <;> simp [op, pcore, unit]
+  intro H; rw [<-H]; simp [disj_empty_l]
+  ext p; rw [in_union]
+  apply Iff.intro
+  · intro H; cases H with | inl H => exfalso; apply in_empty H | inr H => apply H
+  · intro H; right; assumption
+
+theorem pcore_idem : pcore x = some cx → pcore cx ≡ some cx := by
+  rcases x with ⟨x | _⟩ <;> rcases cx with ⟨cx | _⟩ <;> simp [pcore, unit]
+
+theorem pcore_op_mono : pcore x = some cx → ∀ y, ∃ cy, pcore (op x y) ≡ some (op cx cy) := by
+  rcases x with ⟨x | _⟩ <;> simp [pcore] <;> intro H y <;> rw [<-H]
+  <;> (exists unit; simp only [unit, op, disj_empty_l, ↓reduceIte, union_empty_l.left_id])
+
+def extend (H : x ≡{n}≡ op y₁ y₂) :
+    Σ' z₁ z₂, x ≡ op z₁ z₂ ∧ z₁ ≡{n}≡ y₁ ∧ z₂ ≡{n}≡ y₂ := by
+  exists y₁, y₂
+
+theorem unit_left_id : op unit x ≡ x := by
+  rcases x with ⟨x | _⟩ <;> simp [op, unit, disj_empty_l, union_empty_l.left_id]
+
+theorem pcore_unit : pcore unit ≡ some unit := by
+  simp [pcore, unit]
+
+instance : CMRA CoPsetDisjO where
+  pcore := pcore
+  op := op
+  ValidN := validN
+  Valid := valid
+  op_ne := op_ne
+  pcore_ne := pcore_ne
+  validN_ne := validN_ne
+  valid_iff_validN := valid_iff_validN
+  validN_succ := validN_succ
+  validN_op_left := validN_op_left
+  assoc := assoc
+  comm := comm
+  pcore_op_left := pcore_op_left
+  pcore_idem := pcore_idem
+  pcore_op_mono := pcore_op_mono
+  extend _ := extend
+
+instance : UCMRA CoPsetDisjO where
+  unit := unit
+  unit_valid := unit_valid
+  unit_left_id := unit_left_id
+  pcore_unit := pcore_unit
+
+theorem copset_disj_included (X Y : CoPset) :
+   copset X ≼ copset Y ↔ X ⊆ Y := by
+  simp only [CMRA.Included]
+  apply Iff.intro
+  · intro ⟨Z, HZ⟩
+    rcases Z with ⟨Z | _⟩
+    · if H : X ## Z
+      then
+        simp [CMRA.op, op, H] at HZ
+        rw [HZ]
+        intro p Hp; rw [in_union]; left; exact Hp
+      else
+        simp [CMRA.op, op, H] at HZ
+    · simp [CMRA.op, op] at HZ
+  · intro Hsub
+    exists copset (Y \ X)
+    have H : X ## (Y \ X) := by
+      intro p H1 H2
+      rw [in_diff] at H2
+      apply H2.right H1
+    simp [CMRA.op, op, H]
+    ext p; rw [in_union, in_diff]
+    apply Iff.intro
+    · intro G
+      cases H : (decide (p ∈ X)) with
+      | true =>
+        simp only [decide_eq_true_eq] at H
+        left; exact H
+      | false =>
+        simp only [decide_eq_false_iff_not] at H
+        right; exact ⟨G, H⟩
+    · rintro (G|G)
+      · apply Hsub _ G
+      · apply G.left
+
+theorem copset_disj_union (X Y : CoPset) (Hdisj : X ## Y) :
+  (copset X) • (copset Y) ≡ copset (X ∪ Y) := by
+  simp [CMRA.op, op]
+  exact Hdisj
+
+theorem copset_disj_valid_op (X Y : CoPset) :
+    ✓ ((copset X) • (copset Y)) ↔ X ## Y := by
+  simp [CMRA.op, op, CMRA.Valid, valid]
+  by_cases H : X ## Y <;> simp [H]
+
+theorem copset_disj_valid_inv_l (X : CoPset) (Y : CoPsetDisjO) :
+    ✓ ((copset X) • Y) → ∃ Y', Y = copset Y' ∧ X ## Y' := by
+  simp [CMRA.op, op, CMRA.Valid, valid]
+  rcases Y with ⟨Y | _⟩ <;> simp <;> by_cases H : X ## Y <;> simp [H]
+
+end CoPset
