src/Iris/Std/FiniteSetInst.lean
@@ -1,0 +1,130 @@
+/-
+Copyright (c) 2026 Sergei Stepanenko. All rights reserved.
+Released under Apache 2.0 license as described in the file LICENSE.
+-/
+
+import Iris.Std.FiniteSet
+import Std.Data.ExtHashSet
+import Std.Data.ExtTreeSet
+
+/-! ## LawfulSet Instances
+
+This file provides `LawfulSet` instances for Lean's standard library set implementations:
+
+* `ExtTreeSet`
+* `ExtHashSet`
+
+These instances allow these types to be used with the abstract set interface
+defined in `FiniteSet.lean`.
+-/
+
+namespace Iris.Std
+
+open Iris.Std.Set
+
+/-! ### ExtHashSet Instance -/
+
+namespace ExtHashSet
+
+variable {α : Type _} [BEq α] [Hashable α] [EquivBEq α] [LawfulHashable α]
+
+instance : Union (Std.ExtHashSet α) where
+  union := Std.ExtHashSet.union
+
+instance : Inter (Std.ExtHashSet α) where
+  inter := Std.ExtHashSet.inter
+
+instance : SDiff (Std.ExtHashSet α) where
+  sdiff := Std.ExtHashSet.diff
+
+instance : Filter α (Std.ExtHashSet α) where
+  filter s φ := Std.ExtHashSet.filter φ s
+
+instance : Set (Std.ExtHashSet α) α where
+
+instance [LawfulBEq α] :
+    LawfulSet (Std.ExtHashSet α) α where
+  ext X Y h := Std.ExtHashSet.ext_mem h
+  mem_empty := Std.ExtHashSet.not_mem_empty
+  singleton_insert := Std.ExtHashSet.singleton_eq_insert.symm
+  mem_insert_eq := by
+    intro s x y heq
+    subst heq
+    exact Std.ExtHashSet.mem_insert_self
+  mem_insert_ne := by
+    intro s x y hne
+    simp; grind only
+  mem_union := Std.ExtHashSet.mem_union_iff
+  mem_inter := Std.ExtHashSet.mem_inter_iff
+  mem_diff := Std.ExtHashSet.mem_diff_iff
+  mem_filter := by
+    intro X φ x
+    simp only [Filter.filter, Std.ExtHashSet.mem_filter]
+    constructor
+    · intro ⟨h1, h2⟩; simp at h2; exact ⟨h1, h2⟩
+    · intro ⟨h1, h2⟩; simp; exact ⟨h1, h2⟩
+
+-- {1, 2} = {2, 1}, yet hash set doesn't have a canonical ordering. interface should output lists quoted by permutation
+-- instance : FiniteSet (Std.ExtHashSet α) α where
+
+end ExtHashSet
+
+/-! ### ExtTreeSet Instance -/
+
+namespace ExtTreeSet
+
+variable {α : Type _} {cmp : α → α → Ordering} [Std.TransCmp cmp]
+
+instance : Union (Std.ExtTreeSet α cmp) where
+  union := Std.ExtTreeSet.union
+
+instance : Inter (Std.ExtTreeSet α cmp) where
+  inter := Std.ExtTreeSet.inter
+
+instance : SDiff (Std.ExtTreeSet α cmp) where
+  sdiff := Std.ExtTreeSet.diff
+
+instance : Filter α (Std.ExtTreeSet α cmp) where
+  filter s φ := Std.ExtTreeSet.filter φ s
+
+instance : Set (Std.ExtTreeSet α cmp) α where
+
+instance [Std.LawfulEqCmp cmp] :
+    LawfulSet (Std.ExtTreeSet α cmp) α where
+  ext X Y h := Std.ExtTreeSet.ext_mem h
+  mem_empty := Std.ExtTreeSet.not_mem_empty
+  singleton_insert := Std.ExtTreeSet.singleton_eq_insert
+  mem_insert_eq := by
+    intro s x y heq
+    subst heq
+    exact Std.ExtTreeSet.mem_insert_self
+  mem_insert_ne := by
+    intro s x y hne
+    simp; grind only
+  mem_union := Std.ExtTreeSet.mem_union_iff
+  mem_inter := Std.ExtTreeSet.mem_inter_iff
+  mem_diff := Std.ExtTreeSet.mem_diff_iff
+  mem_filter := by
+    intro X φ x
+    simp only [Filter.filter, Std.ExtTreeSet.mem_filter]
+    constructor
+    · intro ⟨h1, h2⟩; simp at h2; exact ⟨h1, h2⟩
+    · intro ⟨h1, h2⟩; simp; exact ⟨h1, h2⟩
+
+instance : FiniteSet (Std.ExtTreeSet α cmp) α where
+  toList s := s.toList
+
+instance [Std.LawfulEqCmp cmp] : LawfulFiniteSet (Std.ExtTreeSet α cmp) α where
+  mem_toList := Std.ExtTreeSet.mem_toList
+  toList_noDup := by
+    intro m
+    have e := Std.ExtTreeSet.distinct_toList (t := m)
+    simp only [List.Nodup]
+    have heq : (fun x1 x2 => x1 ≠ x2) = (fun a b => ¬cmp a b = Ordering.eq) := by
+      ext x1 x2; simp
+    rw [heq]
+    apply e
+
+end ExtTreeSet
+
+end Iris.Std
